cfrontend/SimplExprspec.v
@@ -38,7 +38,7 @@ Section SPEC.
   (* =dest_below_iprop= *)
 Definition dest_below (dst: destination) : iProp :=
   match dst with
-  | For_set sd => IsFresh (sd_temp sd)
+  | For_set sd => & (sd_temp sd)
   | _ => emp
   end.
   (* =end= *)
@@ -54,7 +54,7 @@ Definition dest_below (dst: destination) : iProp :=
   Definition tr_rvalof (ty : type) (e1 : expr) (ls : list statement) (e : expr) : iProp :=
     if type_is_volatile ty
     then
-      (∃ t, ⌜ ls = make_set t e1 :: nil /\ e = Etempvar t ty⌝ ∗ IsFresh t)%I
+      (∃ t, ⌜ ls = make_set t e1 :: nil /\ e = Etempvar t ty⌝ ∗ & t)%I
     else
       ⌜ls =nil /\ e = e1⌝%I.
   (* =tr_expr_iprop= *)
@@ -180,7 +180,7 @@ Fixpoint tr_expr (*[*)(le : temp_env)(*]*) (dst : destination) (*[*)(e : Csyntax
       ∃ (*[*)sl2 a2 sl3 a3 (*]*)t,
        tr_expr (*[*)le For_val e1 sl2 a2(*]*) ∗
        tr_expr (*[*)le For_val e2 sl3 a3 (*]*)∗
-       IsFresh t ∗
+       & t ∗
        dest_below dst ∗
        ⌜ (*[*)sl = sl2 ++ sl3 ++ Sset t (Ecast a3 (Csyntax.typeof e1)) ::
                        make_assign a2 (Etempvar t (Csyntax.typeof e1)) ::
@@ -206,7 +206,7 @@ Fixpoint tr_expr (*[*)(le : temp_env)(*]*) (dst : destination) (*[*)(e : Csyntax
        tr_expr le For_val e1 sl2 a2  ∗
        tr_expr le For_val e2 sl3 a3  ∗
        tr_rvalof (Csyntax.typeof e1) a2 sl4 a4  ∗
-       IsFresh t ∗
+       & t ∗
        ⌜ sl = sl2 ++ sl3 ++ sl4 ++ Sset t (Ecast (Ebinop ope a4 a3 tyres) (Csyntax.typeof e1)) :: make_assign a2 (Etempvar t (Csyntax.typeof e1)) :: final dst (Etempvar t (Csyntax.typeof e1))
        /\ a = Etempvar t (Csyntax.typeof e1) ⌝
      end
@@ -220,7 +220,7 @@ Fixpoint tr_expr (*[*)(le : temp_env)(*]*) (dst : destination) (*[*)(e : Csyntax
        ⌜ sl = sl2 ++ sl3 ++ make_assign a2 (transl_incrdecr id a3 (Csyntax.typeof e1)) :: nil ⌝
     | _ =>
       dest_below dst ∗
-      ∃ t, IsFresh t  ∗
+      ∃ t, & t  ∗
       ⌜ sl = sl2 ++ make_set t a2 ::make_assign a2 (transl_incrdecr id (Etempvar t (Csyntax.typeof e1)) (Csyntax.typeof e1)) :: final dst (Etempvar t (Csyntax.typeof e1))
            /\ a = Etempvar t (Csyntax.typeof e1)⌝
      end
@@ -240,7 +240,7 @@ Fixpoint tr_expr (*[*)(le : temp_env)(*]*) (dst : destination) (*[*)(e : Csyntax
        ⌜  sl = sl2 ++ sl3 ++ Scall None a2 al3 :: nil ⌝
     | _ =>
       dest_below dst ∗ ∃ sl2 a2 sl3 al3 t,
-       IsFresh t ∗
+       & t ∗
         tr_expr le For_val e1 sl2 a2  ∗
         tr_exprlist le el2 sl3 al3  ∗
         ⌜ sl = sl2 ++ sl3 ++ Scall (Some t) a2 al3 :: final dst (Etempvar t ty) /\
@@ -256,7 +256,7 @@ Fixpoint tr_expr (*[*)(le : temp_env)(*]*) (dst : destination) (*[*)(e : Csyntax
     | _ =>
       dest_below dst ∗ ∃ sl2 al2 t,
        tr_exprlist le el sl2 al2  ∗
-       IsFresh t  ∗
+       & t  ∗
        ⌜ sl = sl2 ++ Sbuiltin (Some t) ef tyargs al2 :: final dst (Etempvar t ty) /\
        a = Etempvar t ty⌝
      end
